Tidy up candle_prover_semanticsScript.sml
There are some existing definitions (the basis decls, the candle decls,
etc.) that can be used. The main theorem is still cheated in the
diverging case, and there is a cheat about the candle kernel environment being
env_ok. The state_ok proof is cheated until the translator is set up to
reveal the contents of simple references from the basis (which should all be
ok).

candle/prover/candle_prover_semanticsScript.sml
@@ -8,34 +8,16 @@ open semanticPrimitivesTheory semanticPrimitivesPropsTheory
      sptreeTheory ml_hol_kernelProgTheory
 open permsTheory candle_kernel_funsTheory candle_kernel_valsTheory
      candle_prover_invTheory candle_prover_evaluateTheory ast_extrasTheory
-     semanticsTheory;
-open ml_translatorLib;
+     candle_basis_evaluateTheory semanticsTheory;
+open holKernelProofTheory basisProgTheory ml_hol_kernelProgTheory;
+open ml_translatorLib ml_progTheory;
 local open ml_progLib in end
 
 val _ = new_theory "candle_prover_semantics";
 
 val _ = translation_extends "ml_hol_kernelProg";
 
-val _ = max_print_depth := 1;
-
-val prog_thm = get_ml_prog_state ()
-  |> ml_progLib.clean_state
-  |> ml_progLib.remove_snocs
-  |> ml_progLib.get_thm
-  |> SIMP_RULE std_ss [ml_progTheory.ML_code_def, ml_progTheory.ML_code_env_def]
-
-Definition basis_and_kernel_def:
-  basis_and_kernel = ^(concl prog_thm |> rator |> rator |> rand)
-End
-
-Overload basis_and_kernel_env = (prog_thm |> concl |> rator |> rand);
-Overload basis_and_kernel_state = (prog_thm |> concl |> rand |> rator);
-
-Theorem Decls_basis_kernel = REWRITE_RULE [GSYM basis_and_kernel_def] prog_thm;
-
-val _ = max_print_depth := 100;
-
-Theorem LPREFIX_lemma[local]:
+Theorem LPREFIX_LNTH:
   ∀n xs l ll.
     LPREFIX xs l ∧
     LNTH n xs = NONE ∧
@@ -45,20 +27,6 @@ Proof
   Induct \\ rpt Cases \\ rw [llistTheory.fromList_def]
   \\ gvs [LPREFIX_LCONS, SF SFY_ss]
 QED
-
-(*
-THM ctxt th
-(ctxt,hyps) |- concl th
-            |=
- *)
-
-(* TODO Print context updates on FFI
-    -- Magnus: actually, we might want to print the entire context
-               for each theorem to make soundness statement simple *)
-
-(*
-  basis_and_kernel = basis ++ candle kernel
- *)
 
 (* TODO move to evaluateProps (or wherever evaluate_decs_cons is)
  *)
@@ -81,25 +49,7 @@ Proof
   \\ rpt CASE_TAC \\ gs []
 QED
 
-(* TODO: 'ffi *)
-
-(*
- |- state_ok ctxt s1
- |- env_ok ctxt (extend_dec_env basis_and_kernel_env init_env)
- *)
-
-Theorem state_ok_init_context:
-  ffi.io_events = [] ⇒
-  state_ok init_context (basis_and_kernel_state ffi)
-Proof
-  cheat
-QED
-
-Theorem env_ok_init_context:
-  env_ok init_context basis_and_kernel_env
-Proof
-  cheat
-QED
+(* TODO move *)
 
 Theorem env_ok_extend_dec_env:
   env_ok ctxt env1 ∧
@@ -109,8 +59,182 @@ Proof
   rw [env_ok_def, extend_dec_env_def, nsLookup_nsAppend_some] \\ gs [SF SFY_ss]
 QED
 
+(* -------------------------------------------------------------------------
+ * - The basis program:
+ *   basis, basis_env, basis_state
+ * - The candle program (includes the former):
+ *   candle_code, candle_init_env, candle_init_state
+ * ------------------------------------------------------------------------- *)
+
+Overload basis_env = (basis_Decls_thm |> concl |> rator |> rand);
+
+Overload basis_state = (basis_Decls_thm |> concl |> rand |> rator);
+
+(* -------------------------------------------------------------------------
+ * Show that the basis program satisfies post_state_ok, simple_dec and
+ * safe_dec. Use this to show basis_env is env_ok.
+ * ------------------------------------------------------------------------- *)
+
+Theorem post_state_ok_basis_state:
+  post_state_ok (basis_state ffi)
+Proof
+  rw [post_state_ok_def, kernel_types_def, kernel_locs_def,
+      the_type_constants_def, the_term_constants_def,
+      the_axioms_def, the_context_def]
+  \\ EVAL_TAC \\ gs []
+QED
+
+Theorem basis_decs_ok:
+  EVERY simple_dec basis ∧
+  EVERY safe_dec basis
+Proof
+  once_rewrite_tac [basis_def]
+  \\ conj_tac
+  \\ EVAL_TAC
+  \\ simp [namespaceTheory.id_to_n_def]
+QED
+
+Theorem env_ok_basis_env:
+  env_ok ctxt basis_env
+Proof
+  assume_tac basis_Decls_thm
+  \\ gs [Decls_def]
+  \\ drule_then (qspec_then ‘ctxt’ mp_tac) evaluate_basis_v_ok_decs
+  \\ simp [basis_decs_ok, post_state_ok_basis_state, env_ok_init_env]
+  \\ rw [env_ok_def, extend_dec_env_def, nsLookup_nsAppend_some, SF SFY_ss]
+QED
+
+(* --------------------------------------------------------------------------
+ * Show that the candle_init_state is state_ok.
+ * ------------------------------------------------------------------------- *)
+
+Definition init_refs_def:
+  init_refs = <|
+      the_type_constants := init_type_constants;
+      the_term_constants := init_term_constants;
+      the_axioms         := init_axioms;
+      the_context        := init_context |>
+End
+
+Theorem STATE_init_refs:
+  STATE init_context init_refs
+Proof
+  simp [STATE_def, CONTEXT_def, init_type_constants_def, init_axioms_def,
+        init_term_constants_def, init_context_def, init_refs_def,
+        holSyntaxTheory.init_ctxt_def, holSyntaxTheory.extends_def]
+QED
+
+Theorem candle_init_state_stamp:
+  n ∈ kernel_types ⇒ n < (candle_init_state ffi).next_type_stamp
+Proof
+  EVAL_TAC \\ gs []
+QED
+
+Theorem kernel_refs_distinct[local,simp]:
+  the_type_constants ≠ the_term_constants ∧
+  the_type_constants ≠ the_axioms ∧
+  the_type_constants ≠ the_context ∧
+  the_term_constants ≠ the_axioms ∧
+  the_term_constants ≠ the_context ∧
+  the_axioms ≠ the_context
+Proof
+  simp [the_type_constants_def, the_term_constants_def, the_context_def,
+        the_axioms_def]
+QED
+
+Theorem LLOOKUPs[local]:
+  (Loc loc = the_type_constants ⇒
+     LLOOKUP (candle_init_state ffi).refs loc =
+     SOME (Refv init_type_constants_v)) ∧
+  (Loc loc = the_term_constants ⇒
+     LLOOKUP (candle_init_state ffi).refs loc =
+     SOME (Refv init_term_constants_v)) ∧
+  (Loc loc = the_axioms ⇒
+     LLOOKUP (candle_init_state ffi).refs loc =
+     SOME (Refv init_axioms_v)) ∧
+  (Loc loc = the_context ⇒
+     LLOOKUP (candle_init_state ffi).refs loc =
+     SOME (Refv init_context_v))
+Proof
+  rpt strip_tac
+  \\ gvs [the_type_constants_def, the_term_constants_def, the_axioms_def,
+          the_context_def]
+  \\ rw [candle_init_state_def, LLOOKUP_EQ_EL, EL_APPEND_EQN]
+QED
+
+Theorem candle_init_state_refs:
+  loc ∈ kernel_locs ⇒
+    kernel_loc_ok init_refs loc (candle_init_state ffi).refs
+Proof
+  gvs [kernel_locs_def, kernel_loc_ok_def]
+  \\ rw [] \\ gs []
+  \\ FIRST (map (drule_then (qspec_then ‘ffi’ assume_tac))
+                (CONJUNCTS LLOOKUPs))
+  \\ first_assum (irule_at Any) \\ gs []
+  \\ simp [init_refs_def, init_type_constants_v_thm, init_term_constants_v_thm,
+           init_axioms_v_thm, init_context_v_thm]
+QED
+
+Theorem candle_init_state_eval[simp]:
+  eval_state_ok (candle_init_state ffi).eval_state
+Proof
+  EVAL_TAC
+QED
+
+Theorem candle_init_state_ffi[simp]:
+  (candle_init_state ffi).ffi = ffi
+Proof
+  EVAL_TAC
+QED
+
+Theorem candle_init_state_state_ok:
+  ffi.io_events = [] ⇒
+  state_ok init_context (candle_init_state ffi)
+Proof
+  strip_tac
+  \\ simp [state_ok_def, candle_init_state_stamp]
+  \\ irule_at Any STATE_init_refs
+  \\ simp [candle_init_state_refs]
+  (* TODO:
+   *    The rest of the state; it's all OK but we cant inspect the references
+   *    until the translator is set up to store defintions. *)
+  \\ rw [LLOOKUP_EQ_EL, EL_APPEND_EQN, candle_init_state_def]
+  \\ gvs [NOT_LESS, LESS_OR_EQ, ref_ok_def, kernel_locs_def,
+          the_context_def, the_axioms_def, the_type_constants_def,
+          the_term_constants_def]
+  \\ cheat
+QED
+
+(* --------------------------------------------------------------------------
+ * Show that candle_init_env is env_ok wrt. the initial context.
+ * ------------------------------------------------------------------------- *)
+
+Theorem candle_init_env_env_ok:
+  env_ok init_ctxt candle_init_env
+Proof
+  cheat
+QED
+
+(* --------------------------------------------------------------------------
+ * Top-level semantics theorem.
+ * ------------------------------------------------------------------------- *)
+
+(* TODO Print context updates on FFI
+    -- Magnus: actually, we might want to print the entire context
+               for each theorem to make soundness statement simple
+   TODO: Use 'ffi
+ *)
+
+(* TODO why do these both exist? *)
+
+Theorem init_context_init_ctxt[local,simp]:
+  init_ctxt = init_context
+Proof
+  rw [holSyntaxTheory.init_ctxt_def, init_context_def]
+QED
+
 Theorem semantics_thm:
-  semantics_prog (init_state ffi) init_env (basis_and_kernel ++ prog) res ∧
+  semantics_prog (init_state ffi) init_env (candle_code ++ prog) res ∧
   EVERY safe_dec prog ∧
   ffi.io_events = [] ∧
   res ≠ Fail ⇒
@@ -128,10 +252,10 @@ Proof
     gs [semanticsTheory.semantics_prog_def]
     \\ gs [semanticsTheory.evaluate_prog_with_clock_def]
     \\ pairarg_tac \\ gvs []
+    \\ assume_tac candle_prog_thm
     \\ gvs [evaluate_decs_append, CaseEqs ["prod", "semanticPrimitives$result"]]
     >- (
-      assume_tac Decls_basis_kernel
-      \\ gs [ml_progTheory.Decls_def]
+      gs [ml_progTheory.Decls_def]
       \\ dxrule_then (qspec_then ‘k’ mp_tac) evaluate_decs_add_to_clock
       \\ qpat_x_assum ‘evaluate_decs _ _ _ = (s1, Rval _)’ assume_tac
       \\ dxrule_then (qspec_then ‘ck1’ mp_tac) evaluate_decs_add_to_clock
@@ -141,11 +265,11 @@ Proof
                     (el 3 (CONJUNCTS evaluate_v_ok))
       \\ impl_tac
       >- (
-        drule_then assume_tac state_ok_init_context
-        \\ assume_tac env_ok_init_context \\ gs []
+        drule_then assume_tac candle_init_state_state_ok
+        \\ assume_tac candle_init_env_env_ok \\ gs []
         \\ irule_at Any env_ok_extend_dec_env \\ gs [env_ok_init_env]
-        \\ gs [state_ok_def, state_component_equality]
-        \\ first_assum (irule_at Any) \\ gs [] \\ cheat)
+        \\ gs [state_ok_def, semanticPrimitivesTheory.state_component_equality]
+        \\ first_assum (irule_at Any) \\ gs [SF SFY_ss])
       \\ strip_tac
       \\ rename1 ‘combine_dec_result _ res’ \\ Cases_on ‘res’ \\ gs []
       >- (
@@ -156,41 +280,21 @@ Proof
         gs [state_ok_def]
         \\ first_assum (irule_at Any) \\ gs [])
       \\ first_assum (irule_at Any) \\ gs [])
-    \\ assume_tac Decls_basis_kernel
     \\ gs [ml_progTheory.Decls_def]
     \\ dxrule_then (qspec_then ‘k’ mp_tac) evaluate_decs_add_to_clock
     \\ dxrule_then (qspec_then ‘ck1’ mp_tac) evaluate_decs_add_to_clock
-    \\ rw [] \\ gs [AllCaseEqs ()])
+    \\ rw [] \\ gs [CaseEqs ["semanticPrimitives$result"]])
+  \\ gs [semanticsTheory.semantics_prog_def]
+  \\ gs [lprefix_lub_def, PULL_EXISTS, every_LNTH]
+  \\ qabbrev_tac ‘ff : num -> io_event llist =
+                    λk. fromList (FST (evaluate_prog_with_clock
+                                         (init_state ffi) init_env k
+                                         (candle_code ++ prog))).io_events’
+  \\ gs []
   \\ cheat
 (*
 
-
-  ntac 2 strip_tac
-  \\ reverse (Cases_on `res`)
-  \\ fs [semanticsTheory.semantics_prog_def]
-  >- (* Terminate *)
-   (fs [semanticsTheory.evaluate_prog_with_clock_def]
-    \\ pairarg_tac \\ fs []
-    \\ rveq \\ fs []
-    \\ drule kernel_evaluate_decs
-    \\ disch_then drule
-    \\ simp []
-    \\ rw [EVERY_MEM, extract_events_def, MEM_MAP, PULL_EXISTS, MEM_FILTER,
-           CaseEq "io_event"]
-    \\ PURE_CASE_TAC \\ fs [] \\ rw []
-    \\ fsrw_tac [SATISFY_ss] [])
-     (* Diverge *)
-  \\ fs [lprefix_lub_def, PULL_EXISTS, every_LNTH]
-  \\ rw []
-  \\ qabbrev_tac
-    `ff : num -> io_event llist =
-      \k. fromList (FST
-        (evaluate_prog_with_clock
-          (init_state ffi) init_env k (kernel_decls ++ prog))).io_events`
-  \\ fs []
-  \\ Cases_on `?k v. LNTH n (ff k) = SOME v` \\ fs []
-  >-
-   (first_x_assum (qspec_then `k` assume_tac)
+    first_x_assum (qspec_then `k` assume_tac)
     \\ first_x_assum (qspec_then `k` strip_assume_tac)
     \\ imp_res_tac LPREFIX_LNTH
     \\ pop_assum kall_tac
@@ -205,7 +309,8 @@ Proof
     \\ first_x_assum irule
     \\ fs [LNTH_fromList]
     \\ drule EL_MEM
-    \\ srw_tac [SATISFY_ss] [])
+    \\ srw_tac [SATISFY_ss] []
+
   \\ `!k. LNTH n (ff k) = NONE` by metis_tac [option_nchotomy] \\ fs []
   \\ `F` suffices_by fs [] \\ rw []
   \\ qpat_x_assum `!ub. _ ==> _` mp_tac
@@ -216,3 +321,4 @@ Proof
 QED
 
 val _ = export_theory ();
+
